ConstrainedDecodingFormalization/Lexing.lean
@@ -12,7 +12,6 @@ import Mathlib.Tactic.Linarith
 
 import ConstrainedDecodingFormalization.RegularExpressionsToEpsilonNFA
 import ConstrainedDecodingFormalization.Automata
-import ConstrainedDecodingFormalization.Partition
 
 open List RegularExpression
 
@@ -81,71 +80,284 @@ structure Token (α : Type u) (Γ : Type v) where
   string : List α
 deriving Repr, DecidableEq
 
-def List.terminalSymbols (terminals : List (Terminal α Γ)) : List Γ :=
-  terminals.map (fun t => t.symbol)
-
-def List.sequence {α : Type u} (tokens : List (Token α Γ)) : List Γ :=
-  tokens.map (fun t => t.symbol)
-
 structure LexerSpec (α Γ σ) where
   automaton : FSA α σ
   term: σ → Option Γ
   hterm: ∀ s, s ∈ automaton.accept ↔ (term s).isSome
   term_inj: ∀ s₁ s₂ t, term s₁ = some t ∧ term s₂ = some t → s₁ = s₂
 
-structure LexerSpecification (α Γ σ) where
-  automaton : FSA α σ
-  term_sym : Γ
+def LexerSpec.seq_term (spec: LexerSpec α Γ σ) (seq: List α) : Option Γ :=
+  match spec.automaton.eval seq with
+  | some s => spec.term s
+  | none => none
 
--- A recognizer for a token: returns true if the input is a valid token
-def isToken (specs : List (LexerSpecification α Γ σ)) (xs : List α) : Option Γ :=
-  --letI := Classical.propDecidable
-  specs.findSome? fun s =>
-    if xs ∈ s.automaton.accepts then some s.term_sym else none
+def Lexer (α : Type u) (Γ : Type v) := List (Ch α) -> Option (List (Ch Γ) × List α)
 
--- A predicate for prefix of any token (Note: decidability not proven yet. Will probably need to do something similar as acceptance decidability.)
-def isPrefix (specs : List (LexerSpecification α Γ σ)) (xs : List α) : Prop :=
-  ∃ s ∈ specs, FSA.isPrefix s.automaton xs
+inductive PartialLexRel (spec: LexerSpec α Γ σ)
+  : List (Ch α) → List (Ch Γ) → List α → Prop
+  -- base case
+| nil :
+    PartialLexRel spec
+      [] [] []
+  -- case 1
+| step_eos {w wn tokens unlexed} :
+    PartialLexRel spec w tokens unlexed →
+    -- this nonsense needs to be done to satisfy the eliminator for some reason
+    -- related? https://github.com/leanprover/lean4/issues/9803
+    wn = w ++ [ExtChar.eos] →
+    unlexed ∈ spec.automaton.accepts →
+      PartialLexRel spec wn (tokens ++ [.eos]) []
+  -- case 2
+| step_char_continue {w wn tokens unlexed ch} :
+    PartialLexRel spec w tokens unlexed →
+    wn = w ++ [ExtChar.char ch] →
+    unlexed ++ [ch] ∈ spec.automaton.prefixLanguage →
+      PartialLexRel spec wn tokens (unlexed ++ [ch])
+  -- case 3
+| step_char_commit {w wn tokens unlexed ch t} :
+    PartialLexRel spec w tokens unlexed →
+    wn = w ++ [ExtChar.char ch] →
+    -- next is not in prefix language, but current is in accept
+    unlexed ++ [ch] ∉ spec.automaton.prefixLanguage →
+    some t = spec.seq_term unlexed →
+      PartialLexRel spec wn (tokens ++ [ExtChar.char t]) [ch]
 
+private def PartialLex_trans (spec: LexerSpec α Γ σ) (prev: Option (List (Ch Γ) × List α))
+   (c : Ch α) : Option (List (Ch Γ) × List α) :=
+  match prev with
+  | none => none
+  | some (tokens, unlexed) =>
+    match c with
+    | ExtChar.eos =>
+      if unlexed ∈ spec.automaton.accepts then
+        some (tokens ++ [.eos], [])
+      else
+        none
+    | ExtChar.char ch =>
+      let new_unlexed := unlexed ++ [ch]
+      match spec.automaton.eval new_unlexed with
+      | some σ' => some (tokens, new_unlexed)
+      | none =>
+        let dst := spec.automaton.eval unlexed
+        match dst with
+        | none => none
+        | some σ =>
+          if h : σ ∈ spec.automaton.accept then
+            let term := spec.term σ
+            have h2 := (spec.hterm σ).mp h
+            match hc : term with
+            | some t => some (tokens ++ [ExtChar.char t], [ch])
+            | none => by
+              simp[term] at hc
+              simp_all
+          else
+            none
 
-inductive LexRel (specs : List (LexerSpecification (Ch α) Γ σ)) :
-    List (Ch α) → List (Ch Γ) → List (Ch α) → Prop
-  | empty :
-      LexRel specs [] [] []
+private def PartialLex_seed (spec: LexerSpec α Γ σ) (seed: Option (List (Ch Γ) × List α)) : Lexer α Γ :=
+  fun w => List.foldl (PartialLex_trans spec) seed w
 
-  -- When the next character is EOS, and wr recognizes a token
-  | done {wr ws ts tj} :
-      LexRel specs ws ts wr →
-      isToken specs wr = some tj →
-      LexRel specs (ws ++ [.eos]) (ts ++ [.char tj]) []
+def PartialLex (spec: LexerSpec α Γ σ) : Lexer α Γ :=
+  PartialLex_seed spec (some ([], []))
 
-  -- When next character is NOT EOS:
-  -- (emit) If wr ∈ L(A^j) but (wr ++ c) is no longer a prefix of any token
-  | emit {wr c cs tj T} :
-      c ≠ .eos →
-      isToken specs wr = some tj →
-      ¬ isPrefix specs (wr ++ [c]) →
-      LexRel specs (c :: cs) T [] →
-      LexRel specs (wr ++ c :: cs) (tj :: T) wr
+theorem PartialLex_pruned_eq_PartialLexRel (spec: LexerSpec α Γ σ) (hp: spec.automaton.pruned) :
+    (∀ w tokens unlexed, (PartialLexRel spec w tokens unlexed) → PartialLex_seed spec (some ([], [])) w = some (tokens, unlexed)) ∧
+    (∀ wp ws seed_f seed_s tokens unlexed, (PartialLexRel spec wp seed_f seed_s) ∧ PartialLex_seed spec (some (seed_f, seed_s)) ws = some (tokens, unlexed) → PartialLexRel spec (wp ++ ws) tokens unlexed)
+      := by
+  have hprune := spec.automaton.pruned_prefixLanguage hp
+  have left : (∀ w tokens unlexed, (PartialLexRel spec w tokens unlexed) → PartialLex_seed spec (some ([], [])) w = some (tokens, unlexed)) := by
+    intro w tokens unlexed h
+    induction h
+    case nil =>
+      simp[PartialLex, PartialLex_seed, PartialLex_trans]
+    case step_eos w wn tokens unlexed ih wwn h hacc =>
+      simp[PartialLex, PartialLex_seed, PartialLex_trans] at hacc ⊢
+      simp[wwn, hacc, PartialLex_trans]
+      exact h
+    case step_char_continue w wn tokens unlexed ch ih wwn h hacc =>
+      simp[PartialLex, PartialLex_seed, PartialLex_trans] at hacc ⊢
+      simp[wwn, hacc, PartialLex_trans]
+      cases he: spec.automaton.eval (unlexed ++ [ch]) with
+      | none =>
+        have : unlexed ++ [ch] ∉ spec.automaton.prefixLanguage := by
+          exact Eq.mpr_not (congrFun (id (Eq.symm hprune)) (unlexed ++ [ch])) fun a => a he
+        contradiction
+      | some σ' =>
+        simp at he
+        simp[he]
+    case step_char_commit w wn tokens unlexed ch t ih wwn hni ht hacc =>
+      simp[PartialLex, PartialLex_seed, PartialLex_trans] at hacc ⊢
+      simp[wwn, hacc, PartialLex_trans]
+      cases he: spec.automaton.eval (unlexed ++ [ch]) with
+      | none =>
+        simp[FSA.eval] at he
+        simp[he]
+        simp[LexerSpec.seq_term] at ht
+        split at ht
+        case h_1 st heq =>
+          simp[heq]
+          have : st ∈ spec.automaton.accept := by
+            apply (spec.hterm st).mpr
+            simp[←ht]
+          exists this
+          split
+          <;> simp_all
+        case h_2 heq =>
+          simp[heq] at ht
+      | some σ' =>
+        have : spec.automaton.evalFrom spec.automaton.start (unlexed ++ [ch]) = none := by
+          simp[←hprune] at hni
+          simp[FSA.intermediateLanguage] at hni
+          have : ¬¬ spec.automaton.evalFrom spec.automaton.start (unlexed ++ [ch]) = none := by
+            exact hni
+          exact not_not.mp this
+        simp[this] at he
 
-  -- (extend) If (wr ++ c) is still a valid prefix of some token
-  | extend {wr c cs T} :
-      c ≠ .eos →
-      isPrefix specs (wr ++ [c]) →
-      LexRel specs cs T (wr ++ [c]) →
-      LexRel specs (c :: cs) T wr
+  constructor
+  . exact left
+  . intro wp ws seed_f seed_s tokens unlexed
+    intro h
+    induction ws generalizing wp seed_f seed_s
+    case nil =>
+      simp[PartialLex_seed] at h
+      cases h.left
+      <;> simp_all
+      case step_eos =>
+        have ⟨hl, htokens, _⟩ := h
+        simp[←htokens]
+        exact hl
+      case step_char_continue =>
+        have ⟨hl, htokens, hunlexed⟩ := h
+        simp[←htokens, ←hunlexed]
+        exact hl
+      case step_char_commit =>
+        have ⟨hl, htokens, hunlexed⟩ := h
+        simp[←htokens, ←hunlexed]
+        exact hl
+    case cons ch tail ih =>
+      have my_inductive_seed:= h.left
+      have computable_eq_some := left wp seed_f seed_s my_inductive_seed
+      have h_token_unlexed := h.right
 
-def Lexer (α : Type u) (Γ : Type v) := List α -> Option (List Γ × List α)
+      simp[PartialLex_seed] at h_token_unlexed
+      cases hns : (PartialLex_trans spec (some (seed_f, seed_s)) ch) with
+      | none =>
+        rw[hns] at h_token_unlexed
+        have : foldl (PartialLex_trans spec) none tail = none := by
+          apply List.foldl_fixed'
+          simp[PartialLex_trans]
+        rw[this] at h_token_unlexed
+        contradiction
+      | some qp =>
+        rw[hns] at h_token_unlexed
+        let ⟨step_tokens, step_unlexed⟩ := qp
 
--- Retain the noncomputable version for proofs
-noncomputable def PartialLex (specs :  List (LexerSpecification (Ch α) Γ σ)) (w : List (Ch α)) :
-    Option (List (Ch Γ) × List (Ch α)) :=
-  letI := Classical.propDecidable
-   if h : ∃ out : List (Ch Γ) × List (Ch α), LexRel specs w out.1 out.2 then
-     some (Classical.choose h)
-   else none
+        match ch with
+        | ExtChar.eos =>
+          simp[PartialLex_trans] at hns
 
---instance : DecidableEq (Γ × St P) := by apply instDecidableEqProd
+          have haccept : seed_s ∈ spec.automaton.accepts := by exact hns.left
+          let new_tokens := seed_f ++ [.eos]
+          have step := PartialLexRel.step_eos my_inductive_seed rfl haccept
+          have ihr := ih (wp ++ [ExtChar.eos]) new_tokens []
+          have ihr := by
+            apply ihr
+            constructor
+            exact step
+            simp[PartialLex_seed]
+            simp[←hns.right.left, ←hns.right.right, new_tokens] at h_token_unlexed ⊢
+            exact h_token_unlexed
+          suffices wp ++ ExtChar.eos :: tail = (wp ++ [ExtChar.eos]) ++ tail by
+            rw[this]
+            exact ihr
+          exact append_cons wp ExtChar.eos tail
+        | ExtChar.char ch =>
+          simp[PartialLex_trans] at hns
+          cases hp : spec.automaton.evalFrom spec.automaton.start (seed_s ++ [ch]) with
+          | some σ' =>
+            simp[hp] at hns
+            let new_tokens := seed_f
+            let new_unlexed := seed_s ++ [ch]
+
+            have hint : (seed_s ++ [ch] ∈ spec.automaton.intermediateLanguage) := by
+              simp [FSA.intermediateLanguage]
+              rw[Set.mem_setOf]
+              simp [hp]
+            have hpfx : (seed_s ++ [ch] ∈ spec.automaton.prefixLanguage) := by
+              rw[←hprune]
+              exact hint
+            have ihr := ih (wp ++ [ExtChar.char ch]) new_tokens new_unlexed
+            have ihr := by
+              apply ihr
+              constructor
+              exact PartialLexRel.step_char_continue my_inductive_seed rfl hpfx
+              simp[PartialLex_seed]
+              simp[new_tokens, new_unlexed, hns]
+              exact h_token_unlexed
+            suffices wp ++ ExtChar.char ch :: tail = (wp ++ [ExtChar.char ch]) ++ tail by
+              rw[this]
+              exact ihr
+            exact append_cons wp (ExtChar.char ch) tail
+          | none =>
+            cases ha : spec.automaton.evalFrom spec.automaton.start seed_s with
+            | none => simp[hp, ha] at hns
+            | some σ =>
+              simp[hp, ha] at hns
+
+              have hint : (seed_s ++ [ch] ∉ spec.automaton.intermediateLanguage) := by
+                simp [FSA.intermediateLanguage]
+                rw[Set.mem_setOf]
+                simp [hp]
+              have hpfx : (seed_s ++ [ch] ∉ spec.automaton.prefixLanguage) := by
+                rw[←hprune]
+                exact hint
+
+              have haccept : (seed_s ∈ spec.automaton.accepts) := by
+                have ⟨t, ht⟩ := hns
+                simp[FSA.accepts, FSA.acceptsFrom]
+                rw[Set.mem_setOf]
+                exists σ
+
+              -- quite round about away but works
+              let term := spec.term σ
+              have ⟨t, ht⟩ : ∃ t, term = some t := by
+                have ⟨ha, ht⟩ := hns
+                have h2 := (spec.hterm σ).mp ha
+                match hc: term with
+                | none =>
+                  simp[term] at hc
+                  simp[hc] at h2
+                | some t => exists t
+
+              let new_tokens := seed_f ++ [ExtChar.char t]
+              let new_unlexed := [ch]
+
+              have ihr := ih (wp ++ [ExtChar.char ch]) new_tokens new_unlexed
+              have ihr := by
+                apply ihr
+                constructor
+                apply PartialLexRel.step_char_commit my_inductive_seed
+                simp[PartialLex_seed]
+                exact hpfx
+                simp[term] at ht
+                simp[LexerSpec.seq_term]
+                simp[ha, ht]
+                simp[PartialLex_seed, new_tokens, new_unlexed, hns]
+                have ⟨ha, ht'⟩ := hns
+                split at ht'
+                case h_1 heq =>
+                  have := h_token_unlexed
+                  simp_all
+                  simp[←ht'.left, ←ht'.right] at this ⊢
+                  simp[heq, ht, term] at ht
+                  rw[←ht]
+                  exact this
+                case h_2 heq =>
+                  simp[heq, ht, term] at ht
+              suffices wp ++ ExtChar.char ch :: tail = (wp ++ [ExtChar.char ch]) ++ tail by
+                rw[this]
+                exact ihr
+              exact append_cons wp (ExtChar.char ch) tail
+
 
 /-- Given a lexing automaton `A`, build a character-to-token lexing FST with output over `Γ`
     For the lexing FSA, we'll use the convention that each terminal symbol is attached to an accept state (see Fig. 1) -/
@@ -170,32 +382,121 @@ def BuildLexingFST (spec: LexerSpec α Γ σ) :
       if h : q ∈ F then
         let T := (term q).get <| ((hterm q).mp h)
         some (q0, [T, .eos])
+      else if q = q0 then
+        some (q0, [.eos])
       else
         none
 
   ⟨q0, step, [q0]⟩
 
+def LexingFST_trans_iff_PartialLex (spec: LexerSpec α Γ σ) (h: [] ∉ spec.automaton.accepts) :
+  ∀ w ts,
+      (∀ wr, PartialLex spec w = some (ts, wr) →
+        (∃ q', ((BuildLexingFST spec).eval w = some (q', ts)) ∧
+                (BuildLexingFST spec).eval wr = some (q', []))) ∧
+      (∀ q', (BuildLexingFST spec).eval w = some (q', ts) → ∃ wr, PartialLex spec w = some (ts, wr))
+            := by
+  intro w ts
+  -- evalFrom fold matches lex foldl more nicely induction wise
+  suffices ∀ seed, (∀ wr, PartialLex_seed spec seed w = some (ts, wr) →
+        (∃ q', ((BuildLexingFST spec).evalFrom_fold_seed w seed = some (q', ts)) ∧
+                (BuildLexingFST spec).evalFrom_fold wr = some (q', []))) ∧
+      (∀ q', (BuildLexingFST spec).eval_fold w = some (q', ts) → ∃ wr, PartialLex_seed spec seed w = some (ts, wr)) by
+    simp[FST.eval_fold_eq_eval] at this
+    exact this
 
--- def PartialLexSplit (spec : LexerSpec α Γ σ) (w : List α) :
---     match PartialLex specs (w.map (λ c => ExtChar.char c) ++ [.eos]) with
---     | some (tokens, unlexed) =>
---       -- exists a partition corresponding to the output of partial lex
---       unlexed = [] ∧
---       ∃ p, IsPartition p w ∧ p.length = tokens.length ∧
---         ∀ t ∈ (List.zip tokens p), ∃ spec ∈ specs, t.fst = spec.term_sym ∧ t.snd ∈ spec.automaton.accepts
---     | none =>
---       -- there is no possible partitions in which we can lex it
---       ∀ p, IsPartition p w → ∃ x ∈ p, ∀ lexer ∈ specs, x ∉ lexer.automaton.accepts
---       := by
---   split
---   case h_1 tokens unlexed heq =>
---     simp[PartialLex] at heq
---     rcases heq
---     case intro w1 h =>
---     cases w1
---     case intro w' h' =>
---     cases h'
---     case intro w'' h'' =>
---     sorry
---   case h_2 =>
---     sorry
+  induction w generalizing ts
+  case nil =>
+    simp[FST.eval_fold, FST.evalFrom_fold, FST.evalFrom_fold_seed]
+    apply And.intro
+    . intro wr
+      intro h
+      simp[PartialLex] at h
+      constructor
+      exact h.left
+      simp[h.right]
+    . intro hl
+      simp[PartialLex]
+      exact hl
+  case cons head tail ih =>
+    constructor
+    . intro wr
+      intro h
+      simp[PartialLex] at h
+      rw[List.foldl.eq_def] at h
+
+    . sorry
+namespace Detokenizing
+
+universe x
+variable { V : Type x }
+variable [BEq V]
+
+def BuildDetokenizingFST (tokens: List (Token α V)) : FST V α Unit :=
+  let step := fun _ s =>
+    match tokens.find? λ t => t.symbol == s with
+    | some t => (Unit.unit, t.string)
+    | none => none
+
+  FST.mk Unit.unit step [Unit.unit]
+
+def detokenize (tokens: List (Token α V)) (w : List V) : Option (List α) :=
+  match w with
+  | [] => some []
+  | w' :: ws =>
+    match tokens.find? λ t => t.symbol == w' with
+    | some t => do
+      let res ← detokenize tokens ws
+      t.string ++ res
+    | none => none
+
+theorem detokenizerFST_eq_detokenizer  ( tokens : List (Token α V)) :
+  ∀ ( w : List V ), detokenize tokens w = ((BuildDetokenizingFST tokens).eval w).map Prod.snd := by
+  intro w
+  have lem : ∀ w, detokenize tokens w = ((BuildDetokenizingFST tokens).evalFrom Unit.unit w).map Prod.snd := by
+    intro w
+    induction w
+    case nil =>
+      simp[detokenize, BuildDetokenizingFST, FST.evalFrom]
+    case cons head tail ih =>
+      simp[FST.eval, FST.evalFrom, detokenize]
+      split <;> simp_all
+      case h_1 =>
+        rename_i tt heq
+        conv =>
+          pattern (BuildDetokenizingFST tokens).step 0 head
+          simp[BuildDetokenizingFST]
+        simp[heq]
+        split <;> simp_all
+      case h_2 =>
+        rename_i tt heq
+        conv =>
+          pattern (BuildDetokenizingFST tokens).step 0 head
+          simp[BuildDetokenizingFST]
+        have h : tokens.find? (λ t => t.symbol == head) = none := by
+          apply List.find?_eq_none.mpr
+          intro x hx
+          rw [heq x hx]
+          trivial
+        rw[h]
+        simp
+  exact lem w
+
+theorem detokenizer_comp { σ0 } ( tokens : List (Token α V)) (f : FST α Γ σ0) :
+  ∀ w, ((FST.compose (BuildDetokenizingFST tokens) f).eval w).map Prod.snd =
+    match detokenize tokens w with
+    | some u => (f.eval u).map Prod.snd
+    | none => none := by
+  intro w
+  have := FST.compose_correct (BuildDetokenizingFST tokens) f w
+  rw[this]
+  simp[FST.compose_fun_eval, FST.compose_fun_evalFrom]
+  rw[detokenizerFST_eq_detokenizer]
+  simp[FST.eval]
+  cases h : (BuildDetokenizingFST tokens).evalFrom (BuildDetokenizingFST tokens).start w with
+  | some u =>
+    simp_all[h, Option.map, Prod.snd]
+    cases f.evalFrom f.start u.2 <;> simp_all
+  | none => simp_all
+
+end Detokenizing
