ConstrainedDecodingFormalization/RealizableSequence.lean
@@ -23,79 +23,6 @@ abbrev Output (α : Type u):= List (List α)
 abbrev Re (Γ : Type v) := List (List Γ)
 
 
-namespace Detokenizing
-
-variable [BEq V]
-
-def BuildDetokenizingFST (tokens: List (Token α V)) : FST V α Unit :=
-  let step := fun _ s =>
-    match tokens.find? λ t => t.symbol == s with
-    | some t => (Unit.unit, t.string)
-    | none => none
-
-  FST.mk Unit.unit step [Unit.unit]
-
-def detokenize (tokens: List (Token α V)) (w : List V) : Option (List α) :=
-  match w with
-  | [] => some []
-  | w' :: ws =>
-    match tokens.find? λ t => t.symbol == w' with
-    | some t => do
-      let res ← detokenize tokens ws
-      t.string ++ res
-    | none => none
-
-theorem detokenizerFST_eq_detokenizer  ( tokens : List (Token α V)) :
-  ∀ ( w : List V ), detokenize tokens w = ((BuildDetokenizingFST tokens).eval w).map Prod.snd := by
-  intro w
-  have lem : ∀ w, detokenize tokens w = ((BuildDetokenizingFST tokens).evalFrom Unit.unit w).map Prod.snd := by
-    intro w
-    induction w
-    case nil =>
-      simp[detokenize, BuildDetokenizingFST, FST.evalFrom]
-    case cons head tail ih =>
-      simp[FST.eval, FST.evalFrom, detokenize]
-      split <;> simp_all
-      case h_1 =>
-        rename_i tt heq
-        conv =>
-          pattern (BuildDetokenizingFST tokens).step 0 head
-          simp[BuildDetokenizingFST]
-        simp[heq]
-        split <;> simp_all
-      case h_2 =>
-        rename_i tt heq
-        conv =>
-          pattern (BuildDetokenizingFST tokens).step 0 head
-          simp[BuildDetokenizingFST]
-        have h : tokens.find? (λ t => t.symbol == head) = none := by
-          apply List.find?_eq_none.mpr
-          intro x hx
-          rw [heq x hx]
-          trivial
-        rw[h]
-        simp
-  exact lem w
-
-theorem detokenizer_comp ( tokens : List (Token α V)) (f : FST α Γ σ0) :
-  ∀ w, ((FST.compose (BuildDetokenizingFST tokens) f).eval w).map Prod.snd =
-    match detokenize tokens w with
-    | some u => (f.eval u).map Prod.snd
-    | none => none := by
-  intro w
-  have := FST.compose_correct (BuildDetokenizingFST tokens) f w
-  rw[this]
-  simp[FST.compose_fun_eval, FST.compose_fun_evalFrom]
-  rw[detokenizerFST_eq_detokenizer]
-  simp[FST.eval]
-  cases h : (BuildDetokenizingFST tokens).evalFrom (BuildDetokenizingFST tokens).start w with
-  | some u =>
-    simp_all[h, Option.map, Prod.snd]
-    cases f.evalFrom f.start u.2 <;> simp_all
-  | none => simp_all
-
-end Detokenizing
-
 section Symbols
 
 variable
@@ -156,7 +83,8 @@ def BuildInverseTokenSpannerTable
 
   (re, tinv)
 
-def itst_fst_eq_rs (fst_comp : FST α Γ σ2) : (BuildInverseTokenSpannerTable fst_comp).fst.toFinset = RealizableSequences fst_comp := by sorry
+def itst_fst_eq_rs (fst_comp : FST α Γ σ2) : (BuildInverseTokenSpannerTable fst_comp).fst.toFinset = RealizableSequences fst_comp := by
+  sorry
 
 def itst_snd_eq_itst (fst_comp : FST α Γ σ2) :
     ∀ rs s, ((BuildInverseTokenSpannerTable fst_comp).snd rs s).toFinset = InverseTokenSpannerTable fst_comp rs s := by sorry
