ConstrainedDecodingFormalization/Partition.lean
@@ -1,4 +1,0 @@
-variable { α }
-
-def IsPartition ( parts : List (List α) ) ( base: List α ) :=
-    (∀ part ∈ parts, ¬part.isEmpty) ∧ parts.flatten = base
